RelationalSem.thy
@@ -1,0 +1,283 @@
+section {* What can Happen during a Contract Invocation *}
+
+text {* This section defines a set of sequence of account states that can appeear during an
+invocation of a countract.  The invocation can be a nested reentrancy, but we focus on one
+invocation.  This means we do not look into details of further reentrancy, but just assume 
+that the inner reentrancy keeps the invariant of the contract.  Of course we need to prove
+that the invariant holds for the code, but when we do that we can assume that the inner
+nested calls keep the invariants (we can say we are doing mathematical induction on the depth
+of reentrancy).  *}
+
+theory RelationalSem
+
+imports Main "./Evm"
+
+begin
+
+subsection {* Some Possible Changes on Our Account State *}
+
+text {* The account state might change even when the account's code is not executing. *}
+
+text {* During blocks, the account might gain balances because somebody mines 
+Ether for the account.  The balance might increase also while other contracts execute
+because they might destroy themselves and send their balance to our account.
+The following relation captures this possibility.
+*}
+
+text {* When a transaction finishes, if our contract is marked as killed, it is destroyed. *}
+
+inductive account_state_natural_change :: "account_state \<Rightarrow> account_state \<Rightarrow> bool"
+where
+natural:
+ "old_bal \<le> new_bal \<Longrightarrow>
+  account_state_natural_change
+   \<lparr> account_address = addr
+   , account_storage = str
+   , account_code = code
+   , account_balance = old_bal
+   , account_ongoing_calls = going
+   , account_killed = killed
+   \<rparr>
+   \<lparr> account_address = addr
+   , account_storage = str
+   , account_code = code
+   , account_balance = new_bal
+   , account_ongoing_calls = going
+   , account_killed = killed
+   \<rparr>"
+| cleaned: -- {* This happens only at the end of a transaction, but we don't know
+              the transaction boundaries.  
+              So this can happen at any moment when there are no ongoing calls.  *}
+  "account_state_natural_change
+  \<lparr> account_address = addr
+  , account_storage = str
+  , account_code = code
+  , account_balance = old_bal
+  , account_ongoing_calls = []
+  , account_killed = True
+  \<rparr>
+  (empty_account addr)"
+
+declare account_state_natural_change.simps [simp]
+
+text "When the execution comes back from an external call, the account state might have changed
+arbitrariliy.  Our strategy is to assume that an invariant is kept here; and later prove that
+the invariant actually holds."
+
+inductive account_state_return_change :: "(account_state \<Rightarrow> bool) \<Rightarrow> account_state \<Rightarrow> account_state \<Rightarrow> bool"
+where
+account_return:
+"invariant
+ \<lparr> account_address = addr
+ , account_storage = new_str
+ , account_code = code
+ , account_balance = new_bal
+ , account_ongoing_calls = ongoing
+ , account_killed = killed
+ \<rparr>
+ \<Longrightarrow>
+ account_state_return_change invariant
+ \<lparr> account_address = addr
+ , account_storage = old_str
+ , account_code = code
+ , account_balance = old_bal
+ , account_ongoing_calls = ongoing
+ , account_killed = killed
+ \<rparr>
+ \<lparr> account_address = addr
+ , account_storage = new_str
+ , account_code = code
+ , account_balance = new_bal
+ , account_ongoing_calls = ongoing
+ , account_killed = killed
+ \<rparr>
+ "
+
+declare account_state_return_change.simps [simp]
+
+text "Next we specify which program results might see a return."
+
+fun returnable_result :: "program_result \<Rightarrow> bool"
+where
+  "returnable_result ProgramStepRunOut = False"
+| "returnable_result (ProgramToWorld (ContractCall _) _ _ _) = True"
+| "returnable_result (ProgramToWorld (ContractCreate _) _ _ _) = True"
+| "returnable_result (ProgramToWorld ContractSuicide _ _ _) = False"
+| "returnable_result (ProgramToWorld ContractFail _ _ _) = False"
+  (* because we are not modeling nested calls here, the effect of the nested calls are modeled in
+   * account_state_return_change *)
+| "returnable_result (ProgramToWorld (ContractReturn _) _ _ _) = False"
+| "returnable_result (ProgramInit _) = False"
+| "returnable_result ProgramInvalid = False"
+| "returnable_result ProgramAnnotationFailure = False"
+
+subsection {* A Round of the Game *}
+
+text {* Now we are ready to specify the worlds turn. *}
+
+inductive world_turn :: "(account_state \<Rightarrow> bool) (* The invariant of our contract*)
+                      \<Rightarrow> (account_state * program_result)
+                         (* the account state before the world's move
+                            and the last thing our account did *)
+                      \<Rightarrow> (account_state * variable_env)
+                         (* the account state after the world's move
+                            and the variable environment from which our contract must start.
+                          *)
+                      \<Rightarrow> bool (* a boolean indicating if that is a possible world's move. *)"
+where
+  world_call: -- {* the world might call our contract. *}
+  "
+   build_venv_called old_state callargs next_venv \<Longrightarrow>
+   world_turn I (old_state, ProgramInit callargs) (old_state, next_venv)"
+| world_return: -- {* the world might return to our contract. *}
+  "account_state_return_change I account_state_going_out account_state_back \<Longrightarrow>
+   build_venv_returned account_state_back result new_v \<Longrightarrow>
+   returnable_result program_r \<Longrightarrow>
+   world_turn I (account_state_going_out, program_r)
+                (account_state_pop_ongoing_call account_state_back, new_v)"
+| world_fail: -- {* the world might fail from an account into our contract. *}
+  "account_state_return_change I account_state_going_out account_state_back \<Longrightarrow>
+   build_venv_failed account_state_back = Some new_v \<Longrightarrow>
+   returnable_result result \<Longrightarrow>
+   world_turn I (account_state_going_out, result)
+                (account_state_pop_ongoing_call account_state_back, new_v)"
+
+text {* As a reply, our contract might make a move, or report an annotation failure.*}
+
+inductive contract_turn :: "(account_state * variable_env) \<Rightarrow> (account_state * program_result) \<Rightarrow> bool"
+where
+  contract_to_world:
+  "build_cenv old_account = cenv \<Longrightarrow>
+   program_sem old_venv cenv 
+      (program_length (cenv_program cenv)) steps
+      = ProgramToWorld act st bal opt_v \<Longrightarrow> (* if the program behaves like this *)
+   account_state_going_out (* and if the account state is updated like this*)
+     = update_account_state old_account act st bal opt_v \<Longrightarrow>
+   contract_turn (old_account, old_venv) (* the contract can change the account state like this. *)
+      (account_state_going_out, ProgramToWorld act st bal opt_v)"
+| contract_annotation_failure:
+  "build_cenv old_account = cenv \<Longrightarrow>
+   program_sem old_venv cenv
+      (program_length (cenv_program cenv)) steps = ProgramAnnotationFailure \<Longrightarrow>
+   contract_turn (old_account, old_venv) (old_account, ProgramAnnotationFailure)"
+
+text {* When we combine the world's turn and the contract's turn, we get one round.
+The round is a binary relation over a single set.
+*}
+
+inductive one_round :: "(account_state \<Rightarrow> bool) \<Rightarrow> (account_state * program_result) \<Rightarrow> (account_state * program_result) \<Rightarrow> bool"
+where
+round:
+"world_turn I a b \<Longrightarrow> contract_turn b c \<Longrightarrow> one_round I a c"
+
+subsection {* Repetitions of rounds *}
+
+text {* So, we can repeat rounds and see where they bring us.  *}
+text {* The definition is taken from the book Concrete Semantics, and then modified *}
+inductive star :: "('a \<Rightarrow> 'a \<Rightarrow> bool) \<Rightarrow> 'a \<Rightarrow> 'a \<Rightarrow> bool"
+where
+refl: "star r x x" |
+step: "r x y \<Longrightarrow> star r y z \<Longrightarrow> star r x z"
+
+text {* The repetition of rounds is either zero-times or once and the repetition. *}
+lemma star_case :
+"star r a c \<Longrightarrow>
+ (a = c \<or> (\<exists> b. r a b \<and> star r b c))"
+apply(induction rule: star.induct; auto)
+done
+
+text {* The next lemma is purely for convenience.
+Actually the rounds can go nowhere after this invocation fails.
+*}
+lemma no_entry_fail [dest!]:
+"star (one_round I)
+      (a, ProgramToWorld ContractFail st bal v_opt)
+      (b, c) \<Longrightarrow> b = a \<and> c = ProgramToWorld ContractFail st bal v_opt"
+apply(drule star_case; simp)
+apply(simp add: one_round.simps add: world_turn.simps)
+done
+
+text {* Similarly, the rounds can go nowhere after this invocation returns. *}
+lemma no_entry_return [dest!]:
+"star (one_round I)
+      (a, ProgramToWorld (ContractReturn data) st bal v_opt)
+      (b, c) \<Longrightarrow> b = a \<and> c = ProgramToWorld (ContractReturn data) st bal v_opt"
+apply(drule star_case; simp)
+apply(simp add: one_round.simps add: world_turn.simps)
+done
+
+text {* Also similarly, the rounds can go nowhere after this invocation
+causes our contract to destroy itself.
+*}
+lemma no_entry_suicide [dest!]:
+"star (one_round I)
+      (a, ProgramToWorld ContractSuicide st bal v_opt)
+      (b, c) \<Longrightarrow> b = a \<and> c = ProgramToWorld ContractSuicide st bal v_opt"
+apply(drule star_case; simp)
+apply(simp add: one_round.simps add: world_turn.simps)
+done
+
+text {* And then the rounds can go nowhere after an annotation failure. *}
+lemma no_entry_annotation_failure [dest!]:
+"star (one_round I)
+      (a, ProgramAnnotationFailure)
+      (b, c) \<Longrightarrow> b = a \<and> c = ProgramAnnotationFailure"
+apply(drule star_case; simp)
+apply(simp add: one_round.simps add: world_turn.simps)
+done
+
+subsection {* How to State an Invariant *}
+
+text {* For any invariant @{term I} over account states, now @{term "star (one_round I)"}
+relation shows all possibilities during one invocation, assuming that the
+invariant is kept during external calls\footnote{This assumption about deeper reentrancy should
+be considered as an induction hypothesis.  There has to be a lemma actually perform
+such induction.}.
+The following template traverses the states and proves that the invariant is actually kept
+after every possible round.  Also the template states that no annotation failures happen.
+*}
+
+definition no_assertion_failure_post :: "(account_state \<Rightarrow> bool) \<Rightarrow> (account_state \<times> program_result) \<Rightarrow> bool"
+where
+"no_assertion_failure_post I fin =
+ (I (fst fin) \<and>
+  snd fin \<noteq> ProgramAnnotationFailure)
+"
+
+definition no_assertion_failure :: "(account_state \<Rightarrow> bool) \<Rightarrow> bool"
+where
+"no_assertion_failure (I :: account_state \<Rightarrow> bool) ==
+  (\<forall> addr str code bal ongoing killed callenv.
+    I \<lparr> account_address = addr, account_storage = str, account_code = code,
+        account_balance = bal, account_ongoing_calls = ongoing, account_killed = killed \<rparr> \<longrightarrow>
+  (\<forall> fin. star (one_round I) (
+    \<lparr> account_address = addr, account_storage = str, account_code = code,
+      account_balance = bal, account_ongoing_calls = ongoing, account_killed = killed \<rparr>
+  , ProgramInit callenv) fin \<longrightarrow>
+  no_assertion_failure_post I fin
+ ))"
+
+subsection {* How to State a Pre-Post Condition Pair *}
+
+text {* After proving a theorem of the above form, I might be interested in 
+a more specific case (if the caller is not this particular account, nothing should change).
+For that purpose, here is another template statement.  This contains everything above plus
+an assumption about the initial call, and a conclusion about the state after the invocation.
+*}
+
+definition pre_post_conditions ::
+"(account_state \<Rightarrow> bool) \<Rightarrow> (account_state \<Rightarrow> call_env \<Rightarrow> bool) \<Rightarrow>
+ (account_state \<Rightarrow> call_env \<Rightarrow> (account_state \<times> program_result) \<Rightarrow> bool) \<Rightarrow> bool"
+where
+"pre_post_conditions (I :: account_state \<Rightarrow> bool) (precondition :: account_state \<Rightarrow> call_env\<Rightarrow> bool)
+(postcondition :: (account_state \<Rightarrow> call_env \<Rightarrow> (account_state \<times> program_result) \<Rightarrow> bool)) ==
+  (\<forall> initial_account initial_call. I initial_account \<longrightarrow>
+     precondition initial_account initial_call \<longrightarrow>
+  (\<forall> fin. star (one_round I) (initial_account, ProgramInit initial_call) fin \<longrightarrow>
+  snd fin \<noteq> ProgramAnnotationFailure \<and>
+  (\<forall> fin_observed. account_state_natural_change (fst fin) fin_observed \<longrightarrow>
+  I fin_observed \<and>
+  postcondition initial_account initial_call (fin_observed, snd fin))))
+"
+
+end
